src/cbor/pulse/raw/CBOR.Pulse.Raw.Match.Perm.fst
@@ -37,6 +37,8 @@ decreases r
       cbor_raw_share_array p (Seq.tail c) q cbor_raw_share ();
       PM.seq_list_match_cons_intro (Seq.head c) a (Seq.tail c) q (cbor_match (p /. 2.0R));
       PM.seq_list_match_cons_intro (Seq.head c) a (Seq.tail c) q (cbor_match (p /. 2.0R));
+      rewrite each Seq.cons (Seq.head c) (Seq.tail c) as c;
+      ();
     }
   }
 }
@@ -81,6 +83,8 @@ decreases r
       cbor_raw_share_map r0 p (Seq.tail c) q cbor_raw_share ();
       PM.seq_list_match_cons_intro (Seq.head c) a (Seq.tail c) q (cbor_match_map_entry0 r0 (cbor_match (p /. 2.0R)));
       PM.seq_list_match_cons_intro (Seq.head c) a (Seq.tail c) q (cbor_match_map_entry0 r0 (cbor_match (p /. 2.0R)));
+      rewrite each Seq.cons (Seq.head c) (Seq.tail c) as c;
+      ();
     }
   }
 }
@@ -145,9 +149,9 @@ fn rec cbor_raw_share
       half_mul_l p v.cbor_tagged_payload_perm;
       fold (cbor_match_tagged v (p /. 2.0R) r cbor_match);
       cbor_match_eq_tagged (p /. 2.0R) v r;
+      fold (cbor_match_tagged v (p /. 2.0R) r cbor_match);
       rewrite (cbor_match_tagged v (p /. 2.0R) r cbor_match)
         as (cbor_match (p /. 2.0R) c r);
-      fold (cbor_match_tagged v (p /. 2.0R) r cbor_match);
       rewrite (cbor_match_tagged v (p /. 2.0R) r cbor_match)
         as (cbor_match (p /. 2.0R) c r)
     }
@@ -228,7 +232,7 @@ fn rec cbor_raw_share
 }
 
 ghost
-fn rec cbor_raw_gather_array
+fn rec __cbor_raw_gather_array
   (p1: perm)
   (c: Seq.seq cbor_raw)
   (r1: list raw_data_item)
@@ -256,25 +260,75 @@ ensures
 decreases r1
 {
   match r1 {
-    Nil -> {
-      PM.seq_list_match_nil_elim c r1 (cbor_match p1);
+    [] -> {
+      PM.seq_list_match_nil_elim c [] (cbor_match p1);
       PM.seq_list_match_nil_elim c r2 (cbor_match p2);
       PM.seq_list_match_nil_intro c r1 (cbor_match (p1 +. p2));
     }
     a1 :: q1 -> {
-      PM.seq_list_match_cons_elim c r1 (cbor_match p1);
+      PM.seq_list_match_cons_elim c (a1 :: q1) (cbor_match p1);
       PM.seq_list_match_cons_elim c r2 (cbor_match p2);
-      let a2 = List.Tot.hd r2;
-      let q2 = List.Tot.tl r2;
+      let a2 :: q2 = r2;
       cbor_raw_gather p1 (Seq.head c) a1 p2 a2;
-      cbor_raw_gather_array p1 (Seq.tail c) q1 p2 q2 cbor_raw_gather ();
+      __cbor_raw_gather_array p1 (Seq.tail c) q1 p2 q2 cbor_raw_gather ();
       PM.seq_list_match_cons_intro (Seq.head c) a1 (Seq.tail c) q1 (cbor_match (p1 +. p2));
+      rewrite each Seq.cons (Seq.head c) (Seq.tail c) as c;
+      ()
     }
   }
 }
 
 ghost
-fn rec cbor_raw_gather_map
+fn cbor_raw_gather_array
+  (p1: perm)
+  (c: cbor_array)
+  (r1: raw_data_item {Array? r1})
+  (p2: perm)
+  (r2: raw_data_item {Array? r2})
+  (cbor_raw_gather: (
+    (p1': perm) ->
+    (c': cbor_raw) ->
+    (r1': raw_data_item) ->
+    (p2': perm) ->
+    (r2': raw_data_item { r1' << r1 }) ->
+    stt_ghost unit emp_inames
+      (cbor_match p1' c' r1' ** cbor_match p2' c' r2')
+      (fun _ -> cbor_match (p1' +. p2') c' r1' **
+        pure (r1' == r2')
+      )
+  ))
+  (_: unit)
+requires
+  cbor_match_array c p1 r1 cbor_match **
+  cbor_match_array c p2 r2 cbor_match
+ensures
+  cbor_match_array c (p1 +. p2) r1 cbor_match **
+  pure (r1 == r2)
+decreases r1
+{
+  unfold cbor_match_array c p1 r1 cbor_match;
+  with v1 _pm1. assert S.pts_to c.cbor_array_ptr #_pm1 v1;
+  unfold cbor_match_array c p2 r2 cbor_match;
+  with v2 _pm2. assert S.pts_to c.cbor_array_ptr #_pm1 v1 ** S.pts_to c.cbor_array_ptr #_pm2 v2;
+  (* ^note: asserting the previous one to disambiguate *)
+  assert PM.seq_list_match v1 (Array?.v r1) (cbor_match (p1 `perm_mul` c.cbor_array_payload_perm));
+  assert PM.seq_list_match v2 (Array?.v r2) (cbor_match (p2 `perm_mul` c.cbor_array_payload_perm));
+  S.gather c.cbor_array_ptr #_ #_ #_pm1 #_pm2; // This is @@allow_ambiguous, but we want the permissions added in the right order (sigh)
+  assert (pure (v1 == v2));
+  rewrite each v2 as v1;
+  __cbor_raw_gather_array _ v1 (Array?.v r1) _ _ cbor_raw_gather ();
+  perm_mul_add_l p1 p2 c.cbor_array_array_perm;
+  perm_mul_add_l p1 p2 c.cbor_array_payload_perm;
+  rewrite each (p1 `perm_mul` c.cbor_array_payload_perm +. p2 `perm_mul` c.cbor_array_payload_perm)
+            as ((p1 +. p2) `perm_mul` c.cbor_array_payload_perm);
+  rewrite each (p1 `perm_mul` c.cbor_array_array_perm +. p2 `perm_mul` c.cbor_array_array_perm)
+            as ((p1 +. p2) `perm_mul` c.cbor_array_array_perm);
+  fold cbor_match_array c (p1 +. p2) r1 cbor_match;
+  ();
+}
+
+ghost
+fn rec __cbor_raw_gather_map0
   (r01: raw_data_item)
   (p1: perm)
   (c: Seq.seq cbor_map_entry)
@@ -304,27 +358,79 @@ ensures
 decreases r1
 {
   match r1 {
-    Nil -> {
-      PM.seq_list_match_nil_elim c r1 (cbor_match_map_entry0 r01 (cbor_match (p1)));
+    [] -> {
+      PM.seq_list_match_nil_elim c [] (cbor_match_map_entry0 r01 (cbor_match (p1)));
       PM.seq_list_match_nil_elim c r2 (cbor_match_map_entry0 r02 (cbor_match (p2)));
       PM.seq_list_match_nil_intro c r1 (cbor_match_map_entry0 r01 (cbor_match (p1 +. p2)));
     }
     a1 :: q1 -> {
-      PM.seq_list_match_cons_elim c r1 (cbor_match_map_entry0 r01 (cbor_match (p1)));
+      PM.seq_list_match_cons_elim c (a1 :: q1) (cbor_match_map_entry0 r01 (cbor_match (p1)));
       PM.seq_list_match_cons_elim c r2 (cbor_match_map_entry0 r02 (cbor_match (p2)));
-      let a2 = List.Tot.hd r2;
-      let q2 = List.Tot.tl r2;
-      unfold (cbor_match_map_entry0 r01 (cbor_match p1) (Seq.head c) a1);
+      let a2 :: q2 = r2;
       unfold (cbor_match_map_entry0 r02 (cbor_match p2) (Seq.head c) a2);
+      unfold (cbor_match_map_entry0 r01 (cbor_match p1) (Seq.head c) a1);
       cbor_raw_gather p1 (Seq.head c).cbor_map_entry_key (fst a1) p2 (fst a2);
       cbor_raw_gather p1 (Seq.head c).cbor_map_entry_value (snd a1) p2 (snd a2);
       fold (cbor_match_map_entry0 r01 (cbor_match (p1 +. p2)) (Seq.head c) a1);
-      cbor_raw_gather_map r01 p1 (Seq.tail c) q1 r02 p2 q2 cbor_raw_gather ();
+      __cbor_raw_gather_map0 r01 p1 (Seq.tail c) q1 r02 p2 q2 cbor_raw_gather ();
       PM.seq_list_match_cons_intro (Seq.head c) a1 (Seq.tail c) q1 (cbor_match_map_entry0 r01 (cbor_match (p1 +. p2)));
+      rewrite each Seq.cons (Seq.head c) (Seq.tail c) as c;
+      ();
     }
   }
 }
 
+ghost
+fn cbor_raw_gather_map
+  (p1: perm)
+  (c: cbor_map)
+  (r1: raw_data_item {Map? r1 })
+  (p2: perm)
+  (r2: raw_data_item {Map? r2})
+  (cbor_raw_gather: (
+    (p1': perm) ->
+    (c': cbor_raw) ->
+    (r1': raw_data_item) ->
+    (p2': perm) ->
+    (r2': raw_data_item { r1' << r1 }) ->
+    stt_ghost unit emp_inames
+      (cbor_match p1' c' r1' ** cbor_match p2' c' r2')
+      (fun _ -> cbor_match (p1' +. p2') c' r1' **
+        pure (r1' == r2')
+      )
+  ))
+  (_: unit)
+requires
+  cbor_match_map0 c p1 r1 cbor_match **
+  cbor_match_map0 c p2 r2 cbor_match
+ensures
+  cbor_match_map0 c (p1 +. p2) r1 cbor_match **
+  pure (eq2 #raw_data_item r1 r2)
+decreases r1
+{
+  unfold cbor_match_map0 c p1 r1 cbor_match;
+  with v1 _pm1. assert S.pts_to c.cbor_map_ptr #_pm1 v1;
+  unfold cbor_match_map0 c p2 r2 cbor_match;
+  with v2 _pm2. assert S.pts_to c.cbor_map_ptr #_pm1 v1 ** S.pts_to c.cbor_map_ptr #_pm2 v2;
+  (* ^note: asserting the previous one to disambiguate *)
+  assert PM.seq_list_match v1 (Map?.v r1) (cbor_match_map_entry0 r1 (cbor_match (p1 `perm_mul` c.cbor_map_payload_perm)));
+  assert PM.seq_list_match v2 (Map?.v r2) (cbor_match_map_entry0 r2 (cbor_match (p2 `perm_mul` c.cbor_map_payload_perm)));
+  S.gather c.cbor_map_ptr #_ #_ #_pm1 #_pm2; // This is @@allow_ambiguous, but we want the permissions added in the right order (sigh)
+  assert (pure (v1 == v2));
+  rewrite each v2 as v1;
+  __cbor_raw_gather_map0 r1 _ v1 (Map?.v r1) r2 _ (Map?.v r2) cbor_raw_gather ();
+  perm_mul_add_l p1 p2 c.cbor_map_payload_perm;
+  perm_mul_add_l p1 p2 c.cbor_map_array_perm;
+  rewrite each (p1 `perm_mul` c.cbor_map_payload_perm +. p2 `perm_mul` c.cbor_map_payload_perm)
+            as ((p1 +. p2) `perm_mul` c.cbor_map_payload_perm);
+  rewrite each (p1 `perm_mul` c.cbor_map_array_perm +. p2 `perm_mul` c.cbor_map_array_perm)
+            as ((p1 +. p2) `perm_mul` c.cbor_map_array_perm);
+  fold cbor_match_map0 c (p1 +. p2) r1 cbor_match;
+  ();
+}
+
+(* This function is quite complicated to work with in Pulse. It would
+be good to find a better way of writing this. *)
 ghost
 fn rec cbor_raw_gather
   (p1: perm)
@@ -344,40 +450,41 @@ fn rec cbor_raw_gather
   cbor_match_cases c #p2;
   match c {
     CBOR_Case_String v -> {
-      rewrite (cbor_match p1 c r1)
-        as (cbor_match_string v p1 r1);
-      unfold (cbor_match_string v p1 r1);
-      rewrite (cbor_match p2 c r2)
-        as (cbor_match_string v p2 r2);
-      unfold (cbor_match_string v p2 r2);
+      unfold cbor_match p1 (CBOR_Case_String v) r1;
+      unfold cbor_match p2 (CBOR_Case_String v) r2;
+      let String t1 l1 v1 = r1;
+      let String t2 l2 v2 = r2;
+      unfold cbor_match_string v p1 (String t1 l1 v1);
+      unfold cbor_match_string v p2 (String t2 l2 v2);
       S.gather v.cbor_string_ptr;
+      assert (pure (r1 == r2));
       perm_mul_add_l p1 p2 v.cbor_string_perm;
-      fold (cbor_match_string v (p1 +. p2) r1);
-      rewrite (cbor_match_string v (p1 +. p2) r1)
-        as (cbor_match (p1 +. p2) c r1);
+      fold cbor_match_string v (p1 +. p2) (String t1 l1 v1);
+      fold cbor_match (p1 +. p2) (CBOR_Case_String v) (String t1 l1 v1);
     }
     CBOR_Case_Int v -> {
-      rewrite (cbor_match p1 c r1)
-        as (cbor_match_int v r1);
-      unfold (cbor_match_int v r1);
-      rewrite (cbor_match p2 c r2)
-        as (cbor_match_int v r2);
-      unfold (cbor_match_int v r2);
-      fold (cbor_match_int v r1);
-      rewrite (cbor_match_int v r1)
-        as (cbor_match (p1 +. p2) c r1);
+      unfold cbor_match p1 (CBOR_Case_Int v) r1;
+      unfold cbor_match p2 (CBOR_Case_Int v) r2;
+      let Int64 t1 v1 = r1;
+      let Int64 t2 v2 = r2;
+      unfold cbor_match_int v (Int64 t1 v1);
+      unfold cbor_match_int v (Int64 t2 v2);
+      (* permissions do not show up in cbor_match_int *)
+      fold cbor_match_int v (Int64 t1 v1);
+      fold cbor_match (p1 +. p2) (CBOR_Case_Int v) (Int64 t1 v1);
     }
     CBOR_Case_Simple v -> {
-      rewrite (cbor_match p1 c r1)
-        as (cbor_match_simple v r1);
-      unfold (cbor_match_simple v r1);
-      rewrite (cbor_match p2 c r2)
-        as (cbor_match_simple v r2);
-      unfold (cbor_match_simple v r2);
-      fold (cbor_match_simple v r1);
-      rewrite (cbor_match_simple v r1)
-        as (cbor_match (p1 +. p2) c r1);
+      unfold cbor_match p1 (CBOR_Case_Simple v) r1;
+      unfold cbor_match p2 (CBOR_Case_Simple v) r2;
+      let Simple v1 = r1;
+      let Simple v2 = r2;
+      unfold cbor_match_simple v (Simple v1);
+      unfold cbor_match_simple v (Simple v2);
+      (* permissions do not show up in cbor_match_simple *)
+      fold cbor_match_simple v (Simple v1);
+      fold cbor_match (p1 +. p2) (CBOR_Case_Simple v) (Simple v1);
     }
+    norewrite
     CBOR_Case_Tagged v -> {
       cbor_match_eq_tagged p1 v r1;
       rewrite (cbor_match p1 c r1)
@@ -397,41 +504,22 @@ fn rec cbor_raw_gather
         as (cbor_match (p1 +. p2) c r1);
     }
     CBOR_Case_Array v -> {
-      cbor_match_eq_array p1 v r1;
-      rewrite (cbor_match p1 c r1)
-        as (cbor_match_array v p1 r1 cbor_match);
-      unfold (cbor_match_array v p1 r1 cbor_match);
-      cbor_match_eq_array p2 v r2;
-      rewrite (cbor_match p2 c r2)
-        as (cbor_match_array v p2 r2 cbor_match);
-      unfold (cbor_match_array v p2 r2 cbor_match);
-      S.gather v.cbor_array_ptr;
-      cbor_raw_gather_array _ _ (Array?.v r1) _ _ cbor_raw_gather ();
-      perm_mul_add_l p1 p2 v.cbor_array_array_perm;
-      perm_mul_add_l p1 p2 v.cbor_array_payload_perm;
-      fold (cbor_match_array v (p1 +. p2) r1 cbor_match);
-      cbor_match_eq_array (p1 +. p2) v r1;
-      rewrite (cbor_match_array v (p1 +. p2) r1 cbor_match)
-        as (cbor_match (p1 +. p2) c r1);
+      unfold cbor_match p1 (CBOR_Case_Array v) r1;
+      unfold cbor_match p2 (CBOR_Case_Array v) r2;
+      let Array len1 a1 = r1;
+      let Array len2 a2 = r2;
+      cbor_raw_gather_array p1 v (Array len1 a1) p2 (Array len2 a2) cbor_raw_gather ();
+      fold cbor_match (p1 +. p2) (CBOR_Case_Array v) (Array len1 a1);
     }
     CBOR_Case_Map v -> {
-      cbor_match_eq_map0 p1 v r1;
-      rewrite (cbor_match p1 c r1)
-        as (cbor_match_map0 v p1 r1 cbor_match);
-      unfold (cbor_match_map0 v p1 r1 cbor_match);
-      cbor_match_eq_map0 p2 v r2;
-      rewrite (cbor_match p2 c r2)
-        as (cbor_match_map0 v p2 r2 cbor_match);
-      unfold (cbor_match_map0 v p2 r2 cbor_match);
-      S.gather v.cbor_map_ptr;
-      cbor_raw_gather_map r1 _ _ (Map?.v r1) r2 _ _ cbor_raw_gather ();
-      perm_mul_add_l p1 p2 v.cbor_map_array_perm;
-      perm_mul_add_l p1 p2 v.cbor_map_payload_perm;
-      fold (cbor_match_map0 v (p1 +. p2) r1 cbor_match);
-      cbor_match_eq_map0 (p1 +. p2) v r1;
-      rewrite (cbor_match_map0 v (p1 +. p2) r1 cbor_match)
-        as (cbor_match (p1 +. p2) c r1);
+      unfold cbor_match p1 (CBOR_Case_Map v) r1;
+      unfold cbor_match p2 (CBOR_Case_Map v) r2;
+      let Map len1 a1 = r1;
+      let Map len2 a2 = r2;
+      cbor_raw_gather_map p1 v (Map len1 a1) p2 (Map len2 a2) cbor_raw_gather ();
+      fold cbor_match (p1 +. p2) (CBOR_Case_Map v) (Map len1 a1);
     }
+    norewrite
     CBOR_Case_Serialized_Tagged v -> {
       rewrite (cbor_match p1 c r1)
         as (cbor_match_serialized_tagged v p1 r1);
@@ -445,6 +533,7 @@ fn rec cbor_raw_gather
       rewrite (cbor_match_serialized_tagged v (p1 +. p2) r1)
         as (cbor_match (p1 +. p2) c r1);
     }
+    norewrite
     CBOR_Case_Serialized_Array v -> {
       rewrite (cbor_match p1 c r1)
         as (cbor_match_serialized_array v p1 r1);
@@ -458,6 +547,7 @@ fn rec cbor_raw_gather
       rewrite (cbor_match_serialized_array v (p1 +. p2) r1)
         as (cbor_match (p1 +. p2) c r1);
     }
+    norewrite
     CBOR_Case_Serialized_Map v -> {
       rewrite (cbor_match p1 c r1)
         as (cbor_match_serialized_map v p1 r1);
