src/cbor/pulse/raw/everparse/CBOR.Pulse.Raw.EverParse.Serialized.Base.fst
@@ -73,7 +73,7 @@ fn cbor_match_serialized_array_intro_aux
       (cbor_match_serialized_array res 1.0R r)
       (pts_to_serialized (LowParse.Spec.VCList.serialize_nlist n serialize_raw_data_item) pc #pm v)
 {
-  fold (cbor_match_serialized_payload_array res.cbor_serialized_payload (1.0R `perm_mul` res.cbor_serialized_perm) v);
+  fold (cbor_match_serialized_payload_array pc (1.0R `perm_mul` pm) v);
   fold (cbor_match_serialized_array res 1.0R r);
   ghost fn aux (_: unit)
     requires emp ** cbor_match_serialized_array res 1.0R r
@@ -109,7 +109,7 @@ fn cbor_match_serialized_map_intro_aux
       (cbor_match_serialized_map res 1.0R r)
       (pts_to_serialized (LowParse.Spec.VCList.serialize_nlist n (serialize_nondep_then serialize_raw_data_item serialize_raw_data_item)) pc #pm v)
 {
-  fold (cbor_match_serialized_payload_map res.cbor_serialized_payload (1.0R `perm_mul` res.cbor_serialized_perm) v);
+  fold (cbor_match_serialized_payload_map pc (1.0R `perm_mul` pm) v);
   fold (cbor_match_serialized_map res 1.0R r);
   ghost fn aux (_: unit)
     requires emp ** cbor_match_serialized_map res 1.0R r
